![](_page_0_Picture_0.jpeg)

![](_page_0_Picture_1.jpeg)

# **COMPLEX NUMBERS AND QUADRATIC EQUATIONS**

v*Mathematics is the Queen of Sciences and Arithmetic is the Queen of Mathematics. – GAUSS* v

# **4.1 Introduction**

76 MATHEMATICS

In earlier classes, we have studied linear equations in one and two variables and quadratic equations in one variable. We have seen that the equation *x* 2 + 1 = 0 has no real solution as *x* 2 + 1 = 0 gives *x* 2 = – 1 and square of every real number is non-negative. So, we need to extend the real number system to a larger system so that we can find the solution of the equation *x* 2 = – 1. In fact, the main objective is to solve the equation *ax*<sup>2</sup> + *bx* + *c* = 0, where D = *b* 2 – 4*ac* < 0, which is not possible in the system of real numbers.

![](_page_0_Picture_6.jpeg)

#### **W. R. Hamilton (1805-1865)**

**4.2 Complex Numbers**

Let us denote −1 by the symbol *i*. Then, we have <sup>2</sup> *i* = −1 . This means that *i* is a solution of the equation *x* 2 + 1 = 0.

A number of the form *a* + *ib*, where *a* and *b* are real numbers, is defined to be a

complex number. For example, 2 + *i*3, (– 1) + *i* 3 , 1 4 11 *i* − <sup>+</sup> are complex numbers.

For the complex number *z* = *a* + *ib*, *a* is called the *real part*, denoted by Re *z* and *b* is called the *imaginary part* denoted by Im *z of the complex number z*. For example, if *z* = 2 + *i*5, then Re *z* = 2 and Im *z* = 5.

Two complex numbers *z* 1 = *a* + *ib* and *z* 2 = *c* + *id* are equal if *a* = *c* and *b* = *d*. **Example 1** If 4*x* + *i*(3*x* – *y*) = 3 + *i* (– 6), where *x* and *y* are real numbers, then find the values of *x* and *y*.

**Solution** We have

4*x* + *i* (3*x* – *y*) = 3 + *i* (–6) ... (1)

Equating the real and the imaginary parts of (1), we get

$$4\mathfrak{x} = \mathfrak{z}, \ 3\mathfrak{x} - \mathfrak{y} = -6, \mathfrak{z}$$

which, on solving simultaneously, give 3 4 *x* = and 33 4 *y* = .

# **4.3 Algebra of Complex Numbers**

In this Section, we shall develop the algebra of complex numbers.

**4.3.1** *Addition of two complex numbers* Let *z* 1 = *a* + *ib* and *z* 2 = *c* + *id* be any two complex numbers. Then, the sum *z* 1 + *z* 2 is defined as follows:

*z* 1 + *z*<sup>2</sup> = (*a* + *c*) + *i* (*b* + *d*), which is again a complex number.

For example, (2 + *i*3) + (– 6 +*i*5) = (2 – 6) + *i* (3 + 5) = – 4 + *i* 8

The addition of complex numbers satisfy the following properties:

- (i) *The closure law* The sum of two complex numbers is a complex number, i.e., *z* 1 + *z* 2 is a complex number for all complex numbers *z* 1 and *z* 2 .
- (ii) *The commutative law* For any two complex numbers *z* 1 and *z* 2 , *z* 1 + *z* 2 = *z* 2 + *z*<sup>1</sup>
- (iii) *The associative law* For any three complex numbers *z* 1 , *z* 2 , *z* 3 , (*z* 1 + *z* 2 ) + *z* 3 = *z* 1 + (*z* 2 + *z* 3 ).
- (iv) *The existence of additive identity* There exists the complex number 0 + *i* 0 (denoted as 0), called the *additive identity* or the *zero complex number,* such that, for every complex number *z*, *z* + 0 = *z.*
- (v) *The existence of additive inverse* To every complex number *z* = *a* + *ib*, we have the complex number – *a* + *i*(– *b*) (denoted as – *z*), called the *additive inverse* or *negative of z.* We observe that *z* + (–*z*) = 0 (the additive identity).

**4.3.2** *Difference of two complex numbers* Given any two complex numbers *z* 1 and *z* 2 , the difference *z* 1 – *z* 2 is defined as follows:

*z* 1 – *z* 2 = *z* 1 + (– z<sup>2</sup> ). For example, (6 + 3*i*) – (2 – *i*) = (6 + 3*i*) + (– 2 + *i* ) = 4 + 4*i* and (2 – *i*) – (6 + 3*i*) = (2 – *i*) + ( – 6 – 3*i*) = – 4 – 4*i* **4.3.3** *Multiplication of two complex numbers* Let *z* 1 = *a* + *ib* and *z* 2 = *c* + *id* be any two complex numbers. Then, the product *z* 1 *z* 2 is defined as follows:

*z* 1 *z* 2 = (*ac* – *bd*) + *i*(*ad* + *bc*) For example, (3 + *i*5) (2 + *i*6) = (3 × 2 – 5 × 6) + *i*(3 × 6 + 5 × 2) = – 24 + *i*28

The multiplication of complex numbers possesses the following properties, which we state without proofs.

- (i) **The closure law** The product of two complex numbers is a complex number, the product *z* 1 *z* 2 is a complex number for all complex numbers *z* 1 and *z* 2 .
- (ii) **The commutative law** For any two complex numbers *z* 1 and *z* 2 ,

$$z\_2 = z\_2 | z\_1 |$$

*z*

- 1 (iii) **The associative law** For any three complex numbers *z* 1 , *z* 2 , *z* 3 , (*z* 1 *z* 2 ) *z* 3 = *z* 1 (*z* 2 *z* 3 ).
- (iv) **The existence of multiplicative identity** There exists the complex number 1 + *i* 0 (denoted as 1), called the *multiplicative identity* such that *z.*1 = *z*, for every complex number *z*.
- (v) **The existence of multiplicative inverse** For every non-zero complex number *z* = *a* + *ib* or *a* + *bi*(*a* ≠ 0, b ≠ 0), we have the complex number

2 2 2 2 *a –b <sup>i</sup> a b a b* + + + (denoted by 1 *z* or *z* –1 ), called the *multiplicative inverse* of *z* such that

1 *z.* 1 *z* = (the multiplicative identity).

(vi) **The distributive law** For any three complex numbers *z* 1 , *z* 2 , *z* 3 ,

$$\begin{array}{ll} \text{(a)} \ z\_1 \ (z\_2 + z\_3) = z\_1 \ z\_2 + z\_1 \ z\_3\\ \text{(b)} \ (z\_1 + z\_2) \ z\_3 \end{array}$$

**4.3.4** *Division of two complex numbers* Given any two complex numbers *z* <sup>1</sup>and *z* 2 ,

where <sup>2</sup> *<sup>z</sup>* <sup>≠</sup> <sup>0</sup> , the quotient <sup>1</sup> 2 *z z* is defined by

$$\frac{z\_1}{z\_2} = z\_1 \frac{1}{z\_2}$$

For example, let *z* 1 = 6 + 3*i* and *z* 2 = 2 – *i*

$$\text{Then } \qquad \frac{1}{z\_2} = \left( (6+3i) \times \frac{1}{2-i} \right) = \left( 6+3i \right) \left( \frac{2}{2^2 + \left(-1\right)^2} + i \frac{-\left(-1\right)}{2^2 + \left(-1\right)^2} \right)$$

$$\mathbf{a} = \left(\mathbf{6} + \mathbf{3}i\right)\left(\frac{\mathbf{2} + i}{\mathbf{5}}\right) = \frac{1}{\mathbf{5}}\left[1\mathbf{2} - \mathbf{3} + i\left(\mathbf{6} + \mathbf{6}\right)\right] = \frac{1}{\mathbf{5}}\left(\mathbf{9} + 12i\right)$$

**4.3.5** *Power of i* we know that

$$i^3 = i^2 \\ i = \left(-1\right)i = -i \\ \qquad \qquad i^4 = \left(i^2\right)^2 = \left(-1\right)^2 = 1$$
 
$$i^5 = \left(i^2\right)^2 i = \left(-1\right)^2 i = i, \qquad i^6 = \left(i^2\right)^3 = \left(-1\right)^3 = -1,\text{ etc.}$$
 
$$\text{Also, we have } \qquad i^{-1} = \frac{1}{i} \times \frac{i}{i} = \frac{i}{-1} = -i, \qquad i^{-2} = \frac{1}{i^2} = \frac{1}{-1} = -1,$$
 
$$i^{-3} = \frac{1}{i^3} = \frac{1}{-i} \times \frac{i}{i} = \frac{i}{1} = i, \quad i^{-4} = \frac{1}{i^4} = \frac{1}{-1} = 1.$$
 
$$\text{real. for any integer } k, \; i^{4k} = 1, \; j^{4k+1} = -1, \; j^{4k+3} = -1,$$

In general, for any integer *k*, *i* = 1, *i* <sup>4</sup>*k* + 1 = *i, i*<sup>4</sup>*k* + 2 = –1, *i* <sup>4</sup>*k* + 3 = – *i*

**4.3.6** *The square roots of a negative real number*

Note that *i*<sup>2</sup> = –1 and ( *– i*) 2 = *i*<sup>2</sup> = – 1

Therefore, the square roots of – 1 are *i*, – *i*. However, by the symbol −1, we would mean *i* only.

Now, we can see that *i* and –*i* both are the solutions of the equation *x* 2 + 1 = 0 or *x* 2 = –1.

$$\begin{aligned} \text{Similarly} \qquad \left(\sqrt{3}\,\text{i}\right)^2 &= \left(\sqrt{3}\right)^2 \,\text{i}^2 = 3 \left(-\text{i}\right) = -3 \,\text{i} \\\ \left(-\sqrt{3}\,\text{i}\right)^2 &= \left(-\sqrt{3}\right)^2 \,\text{i}^2 = -3 \end{aligned}$$

Therefore, the square roots of –3 are 3 *i* and − 3*i* .

Again, the symbol −3 is meant to represent 3 *i* only, i.e., −3 = 3 *i* .

Generally, if *a* is a positive real number, −*a* = *a* −1 = *a i* ,

We already know that *a b* × = *ab* for all positive real number *a* and *b*. This result also holds true when either *a* > 0, *b* < 0 or *a* < 0, *b* > 0. What if *a* < 0, *b* < 0? Let us examine.

Note that

$$i^2 = \sqrt{-1} \cdot \sqrt{-1} = \sqrt{(-1)\left(-1\right)} \text{ (by assuming } \sqrt{a} \times \sqrt{b} = \sqrt{ab} \text{ for all real numbers)}.$$

$$= \sqrt{1} = 1, \text{ which is a contradiction to the fact that } i^2 = -1.$$

$$\text{Therefore, } \sqrt{a} \times \sqrt{b} \neq \sqrt{ab} \text{ : if both } a \text{ and } b \text{ are negative real numbers.}$$

$$\text{Further, if any of } a \text{ and } b \text{ is zero, then, clearly, } \sqrt{a} \times \sqrt{b} = \sqrt{ab} = 0.$$

**4.3.7** *Identities* We prove the following identity

( )<sup>2</sup> 2 2 *z z z z z z* 1 2 1 2 1 2 + = + + 2 , for all complex numbers *z* 1 and *z* 2 .

$$\begin{aligned} \text{Proof } \text{ We have,} \quad & \begin{pmatrix} z\_1 + z\_2 \end{pmatrix} = \begin{pmatrix} z\_1 + z\_2 \end{pmatrix} \begin{pmatrix} z\_1 + z\_2 \end{pmatrix}, \\ &= \begin{pmatrix} z\_1 + z\_2 \end{pmatrix} z\_1 + \begin{pmatrix} z\_1 + z\_2 \end{pmatrix} z\_2 \qquad & \text{(Distributive law)} \\ &= z\_1^2 + z\_2 z\_1 + z\_1 z\_2 + z\_2^2 \\ &= z\_1^2 + z\_1 z\_2 + z\_1 z\_2 + z\_2^2 \qquad & \text{(Distributive law of multiplication)} \\ &= z\_1^2 + 2z\_1 z\_2 + z\_2^2 \end{aligned}$$

Similarly, we can prove the following identities:

- (i) ( )<sup>2</sup> <sup>2</sup> <sup>2</sup> *z z z z z z* 1 2 1 1 2 2 − = − + 2 (ii) ( )<sup>3</sup> 3 2 2 3 *z z z z z z z z* 1 2 1 1 2 1 2 2 + = + + + 3 3 (iii) ( )<sup>3</sup> 3 2 2 3 *z z z z z z z z* 1 2 1 1 2 1 2 2 − = − + − 3 3
- (iv) ( ) ( ) 2 2 1 2 1 2 1 2 *z – z z z z – z* = +

In fact, many other identities which are true for all real numbers, can be proved to be true for all complex numbers.

**Example 2** Express the following in the form of *a* + *bi*:

$$\text{(i)} \quad \left(-\right)\left(-5i\right)\left(\frac{1}{8}i\right) \qquad \text{(ii)} \quad \left(-i\right)\left(2i\right)\left(-\frac{1}{8}i\right)^{3}$$

$$\text{Solution} \quad \text{(i)} \quad \left(-5i\right)\left(\frac{1}{8}i\right) = \frac{-5}{8}i^{2} = \frac{-5}{8}(-1) = \frac{5}{8} = \frac{5}{8} + i0$$

$$\text{(ii)} \quad \left(-i\right)\left(2i\right)\left(-\frac{1}{8}i\right)^{3} = 2 \times \frac{1}{8 \times 8 \times 8} \times i^{5} = \frac{1}{256}\left(i^{2}\right)^{2}i = \frac{1}{256}i\dots i$$

**Example 3** Express (5 – 3*i*) <sup>3</sup>in the form *a* + *ib*.

**Solution** We have, (5 – 3*i*) <sup>3</sup> = 5 3 – 3 × 5<sup>2</sup> × (3*i*) + 3 × 5 (3*i*) 2 – (3*i*) 3 = 125 – 225*i* – 135 + 27*i* = – 10 – 198*i.*

**Example 4** Express (− + − − 3 2 2 3 )( *i*)in the form of *a* + *ib*

$$\begin{aligned} \text{Solution We have, } \left( \begin{pmatrix} -\sqrt{3} + \sqrt{-2} \\ \end{pmatrix} \begin{pmatrix} 2\sqrt{3} - i \end{pmatrix} \right) &= \left( -\sqrt{3} + \sqrt{2}i \right) \left( 2\sqrt{3} - i \right) \\ &= \left( -6 + \sqrt{3}i + 2\sqrt{6}i - \sqrt{2}i^2 \right) = \left( -6 + \sqrt{2} \right) + \sqrt{3} \left( 1 + 2\sqrt{2} \right)i \end{aligned}$$

## **4.4 The Modulus and the Conjugate of a Complex Number**

Let *z* = *a* + *ib* be a complex number. Then, the modulus of *z*, denoted by | *z* |, is defined to be the non-negative real number 2 2 *a b* + , i.e., | *z* | = 2 2 *a b* + and the conjugate of *z*, denoted as *z* , is the complex number *a* – *ib*, i.e., *z* = *a* – *ib*.

$$\begin{aligned} \text{For example,} \\ \text{and} \\ \text{and} \end{aligned} \qquad \begin{aligned} \left| \begin{array}{c} 3+i \end{array} \right| = \sqrt{3^2 + 1^2} = \sqrt{10}, \quad \left| \begin{array}{c} 2 - 5i \end{array} \right| = \sqrt{2^2 + (-5)^2} = \sqrt{29}, \\ \text{and} \\ \begin{array}{c} \sqrt{3+i} = 3 - i, \quad \boxed{2-5i} = 2 + 5i, \quad \boxed{3i-5} = 3i - 5 \end{aligned} \end{aligned}$$

Observe that the multiplicative inverse of the non-zero complex number *z* is given by

$$\begin{aligned} z^{-1} &= \frac{1}{a+ib} = \frac{a}{a^2+b^2} + i\frac{-b}{a^2+b^2} = \frac{a-ib}{a^2+b^2} = \frac{\overline{z}}{\left|\frac{z}{z}\right|^2},\\ \frac{1}{z} \overline{\overline{z}} &= \left|z\right|^2 \end{aligned}$$

or *z*

Furthermore, the following results can easily be derived. For any two compex numbers *z* 1 and *z* 2 , we have

$$\begin{array}{c} \text{(i)} \quad \left| \begin{array}{c} z\_1 \\ z\_1 \end{array} z\_2 \right| = \left| z\_1 \right| \left| z\_2 \right| \qquad \text{(ii)} \quad \left| \begin{array}{c} \frac{z\_1}{z\_2} \\ \frac{z\_1}{z\_2} \end{array} \right| = \left| \frac{z\_1}{z\_2} \right| \quad \text{provided} \left| \begin{array}{c} z\_2 \\ \end{array} \right| \neq 0 \\\\ \begin{array}{c} \frac{z\_1}{(z\_2)} \end{array} \end{array}$$

$$\text{(iii)} \quad \overline{z\_1 z\_2} = \overline{z\_1} \overline{z\_2} \qquad \qquad \text{(iv)} \quad \overline{z\_1 \pm z\_2} = \overline{z\_1} \pm \overline{z\_2} \text{ (v)}\\ \left(\frac{z\_1}{z\_2}\right) = \frac{\overline{z\_1}}{\overline{z\_2}} \quad \text{provided } z\_2 \neq 0.$$

#### 82 MATHEMATICS

**Example 5** Find the multiplicative inverse of 2 – 3*i*.

**Solution** Let *z* = 2 – 3*i*

$$\text{Then } \qquad \left| \overline{z} \right| = 2 + 3i \text{ and } \qquad \left| \left| z \right| \right|^2 = 2^2 + (-3)^2 = 13$$

Therefore, the multiplicative inverse of 2 3 − *i* is given by

$$z^{-1} = \frac{\overline{z}}{\left| \left. \overline{z} \right|^2} = \frac{2 + 3i}{13} = \frac{2}{13} + \frac{3}{13}i$$

The above working can be reproduced in the following manner also,

$$z^{-1} = \frac{1}{2 - 3i} = \frac{2 + 3i}{(2 - 3i)(2 + 3i)}$$

$$= \frac{2 + 3i}{2^2 - (3i)^2} = \frac{2 + 3i}{13} = \frac{2}{13} + \frac{3}{13}i$$

**Example 6** Express the following in the form *a* + *ib*

$$\text{(i)}\ \frac{\mathfrak{s} + \sqrt{2}i}{1 - \sqrt{2}i} \qquad\qquad\qquad\qquad\qquad\qquad\qquad\qquad\qquad\qquad\qquad\text{(ii)}\ \frac{i^{3\mathfrak{s}}}{\sqrt{2}}$$

$$\text{Solution} \quad \text{(i)} \quad \text{We have, } \frac{5+\sqrt{2}i}{1+\sqrt{2}i} = \frac{5+\sqrt{2}i}{1-\sqrt{2}i} \times \frac{1+\sqrt{2}i}{1+\sqrt{2}i} = \frac{5+5\sqrt{2}i+\sqrt{2}i-2}{1-\left(\sqrt{2}i\right)^2}$$

$$= \frac{3+6\sqrt{2}i}{1+2} = \frac{3(1+2\sqrt{2}i)}{3} = 1+2\sqrt{2}i$$

$$\text{(ii) } t^{-3} = \frac{1}{t^{3\delta}} = \frac{1}{\left(t^2\right)^{17}i} = \frac{1}{-i} \times \frac{i}{i} = \frac{i}{-i^2} = i$$

$$\text{EXEURISE (4.1)}$$

Express each of the complex number given in the Exercises 1 to 10 in the form *a* + *ib.*

$$\begin{array}{ccccc} \text{1.} & \text{(5i)} \left(-\frac{3}{5}i\right) & \text{(2.)} & \text{i}^{9} + \text{i}^{19} & \text{0.} & \text{i}^{-39} \end{array}$$

$$\begin{array}{cccc} 4. & 3(7+i7)+i\left(7+i7\right) & 5. & (1-i)-(-1+i6) \\\\ 6. & \left(\frac{1}{5}+i\frac{2}{5}\right)-\left(4+i\frac{5}{2}\right) & 7. & \left[\left(\frac{1}{3}+i\frac{7}{3}\right)+\left(4+i\frac{1}{3}\right)\right]-\left(-\frac{4}{3}+i\right) \\\\ 8. & (1-i)^{4} & 9. & \left(\frac{1}{3}+3i\right)^{3} & 10. & \left(-2-\frac{1}{3}i\right)^{3} \end{array}$$

Find the multiplicative inverse of each of the complex numbers given in the Exercises 11 to 13.

- **11.** 4 3*i* **12.** 5 3 + *i* **13.** *i*
- **14.** Express the following expression in the form of *a* + *ib* :

$$\frac{\left(3+i\sqrt{5}\right)\left(3-i\sqrt{5}\right)}{\left(\sqrt{3}+\sqrt{2}\ i\right)-\left(\sqrt{3}-i\sqrt{2}\right)}$$

## **4.5 Argand Plane and Polar Representation**

We already know that corresponding to each ordered pair of real numbers (*x*, *y*), we get a unique point in the XYplane and vice-versa with reference to a set of mutually perpendicular lines known as the *x*-axis and the *y*-axis. The complex number *x* + *iy* which corresponds to the ordered pair (*x*, *y*) can be represented geometrically as the unique point P(*x*, *y*) in the XY-plane and vice-versa.

Some complex numbers such as 2 + 4*i*, – 2 + 3*i*, 0 + 1*i*, 2 + 0*i*, – 5 –2*i* and 1 – 2*i* which correspond to the ordered

![](_page_7_Figure_9.jpeg)

pairs (2, 4), ( – 2, 3), (0, 1), (2, 0), ( –5, –2), and (1, – 2), respectively, have been represented geometrically by the points A, B, C, D, E, and F, respectively in the Fig 4.1.

The plane having a complex number assigned to each of its point is called the *complex plane* or the *Argand plane*.

#### 84 MATHEMATICS

Obviously, in the Argand plane, the modulus of the complex number

*x* + *iy* = 2 2 *x y* + is the distance between the point P(*x*, *y*) and the origin O (0, 0) (Fig 4.2). The points on the *x*-axis corresponds to the complex numbers of the form *a* + *i* 0 and the points on the *y*-axis corresponds to the complex numbers of the form

![](_page_8_Figure_3.jpeg)

0 + *i b*. The *x*-axis and *y*-axis in the Argand plane are called, respectively, the *real axis* and the *imaginary axis*.

The representation of a complex number *z* = *x* + *iy* and its conjugate *z* = *x* – *iy* in the Argand plane are, respectively, the points P (*x, y*) and Q (*x, – y*).

Geometrically, the point (*x*, *– y*) is the mirror image of the point (*x*, *y*) on the real axis (Fig 4.3).

![](_page_8_Figure_7.jpeg)

**Fig 4.3**

## *Miscellaneous Examples*

**Example 7** Find the conjugate of (3 2 )(2 3 ) (1 2 )(2 ) *i i i i* − + + − . **Solution** We have , (3 2 )(2 3 ) (1 2 )(2 ) *i i i i* − + + − = 6 9 4 6 2 4 2 *i i i i* + − + − + + = 12 5 4 3 4 3 4 3 *i i i i* + − × + − = 48 36 20 15 63 16 16 9 25 − + + − *i i i* = + = 63 16 25 25 − *i* Therefore, conjugate of (3 2 )(2 3 ) 63 16 is (1 2 )(2 ) 25 25 *i i <sup>i</sup> i i* − + + + − .

**Example 8** If *x* + *iy* = *a ib a ib* + − , prove that *x* 2 + *y* 2 = 1.

**Solution** We have,

$$\langle x+ib \rangle \equiv \underbrace{\frac{(a+ib)(a+ib)}{(a-ib)(a+ib)}}\_{\phantom{\alpha}} = \frac{\frac{a^2}{a^2} - b^2 + 2ab i}{a^2 + b^2} = \frac{a^2 - b^2}{a^2 + b^2} + \frac{2ab}{a^2 + b^2} i$$

So that, *x* – *iy =*  2 2 2 2 2 2 *a b ab* 2 *i a b a b* − − + +

Therefore,

$$\chi^2 + \chi^2 = (\chi + i\wp)(\chi \pm i\wp) = \frac{(a^2 - b^2)^2}{(a^2 + b^2)^2} + \frac{4a^2b^2}{(a^2 + b^2)^2} = \frac{(a^2 + b^2)^2}{(a^2 + b^2)^2} = 1$$

## *Miscellaneous Exercise on Chapter* **4**

- **1.** Evaluate: 3 25 <sup>18</sup> 1 *i i* <sup>+</sup> .
- **2.** For any two complex numbers *z* 1 and *z* 2 , prove that Re (*z* 1 *z* 2 ) = Re *z* 1 Re *z* 2 – Im*z* 1 Im*z* 2 .

$$\begin{aligned} \text{3. } \quad \text{Reduce } \left(\frac{1}{1-4i}-\frac{2}{1+i}\right)\left(\frac{3-4i}{5+i}\right) \text{ to the standard form } \\\\ \text{4. } \quad \text{If } \ge -i\text{y} = \sqrt{\frac{a-ib}{c-id}} \text{ prove that } \left(\mathbf{x}^2 + \mathbf{y}^2\right)^2 = \frac{a^2+b^2}{c^2+d^2}. \\\\ \text{5. } \quad \text{If } z\_1 = 2-i, z\_2 = 1+i, \text{ find } \left|\frac{z\_1+z\_2+1}{z\_1-z\_2+1}\right|. \\\\ \text{6. } \quad \text{If } a+ib = \frac{\left(\mathbf{x}+i\right)^2}{2\mathbf{x}^2+1}, \text{ prove that } a^2+b^2 = \frac{\left(\mathbf{x}^2+1\right)^2}{\left(2\mathbf{x}^2+1\right)^2}. \\\\ \text{7. } \quad \text{Let } z\_1 = 2-i, z\_2 = -2+i. \text{ Find} \end{aligned}$$

$$\text{(i) } \operatorname{Re}\left(\frac{z\_1 z\_2}{\overline{z}\_1}\right), \qquad\qquad\qquad\text{(ii) } \operatorname{Im}\left(\frac{1}{z\_1^2 \overline{z}\_1}\right)^{-1}$$

**8.** Find the real numbers *x* and *y* if (*x* – *iy*) (3 + 5*i*) is the conjugate of –6 – 24*i*.

$$\textbf{9.}\qquad\text{Find the modulus of }\underbrace{1+i}\_{\text{---}}-\frac{1-i}{1+i}\dots$$

$$10. \quad \text{If } (\mathbf{x} + i\mathbf{y})^3 = \boldsymbol{\mu} + i\mathbf{\hat{v}}, \text{ then show that } \frac{\boldsymbol{\mu}}{\boldsymbol{\lambda}} + \frac{\mathbf{v}}{\mathbf{y}} = 4(\mathbf{x}^2 - \mathbf{y}^2) \cdot \mathbf{\hat{v}}$$

**11.** If α and β are different complex numbers with β 1 = , then find β α 1 αβ *– –* .

- **12.** Find the number of non-zero integral solutions of the equation 1 2 *<sup>x</sup> <sup>x</sup> – i* = .
- **13.** If (*a* + *ib*) (*c* + *id*) (*e* + *if*) (*g* + *ih*) = A + *i*B, then show that (*a* 2 + *b* 2 ) (*c* 2 + *d* 2 ) (*e* 2 + *f* 2 ) (*g* 2 + *h* 2 ) = A<sup>2</sup> + B<sup>2</sup>
- **14.** If 1 1 1 *m i – i* + = , then find the least positive integral value of *m*.

# *Summary*

- ÆA number of the form *a* + *ib*, where *a* and *b* are real numbers, is called a *complex number*, *a* is called the *real part* and *b* is called the *imaginary* part of the complex number.
- ÆLet *z* 1 = *a* + *ib* and *z* 2 = *c* + *id*. Then
	- (i) *z* 1 + *z* 2 = (*a* + *c*) + *i* (*b* + *d*)
	- (ii) *z* 1 *z* 2 = (*ac* – *bd*) + *i* (*ad* + *bc*)

ÆFor any non-zero complex number *z* = *a* + *ib* (*a* ≠ 0, *b* ≠ 0), there exists the

complex number 2 2 2 2 *a b <sup>i</sup> a b a b* − + + + , denoted by 1 *z* or *z* –1, called the

*multiplicative inverse* of *z* such that (*a* + *ib*) 2 2 2 2 − + + + *a b i a b a b* = 1 + *i*<sup>0</sup>

=1

- ÆFor any integer *k*, *i* 4*k* = 1, *i* <sup>4</sup>*k* + 1 = *i*, *i* <sup>4</sup>*k* + 2 = – 1, *i* <sup>4</sup>*k* + 3 = – *i*
- ÆThe conjugate of the complex number *z* = *a* + *ib*, denoted by *z* , is given by *z* = *a* – *ib.*

# *Historical Note*

The fact that square root of a negative number does not exist in the real number system was recognised by the Greeks. But the credit goes to the Indian mathematician *Mahavira* (850) who first stated this difficulty clearly. "He mentions in his work '*Ganitasara Sangraha*' as in the nature of things a negative (quantity) is not a square (quantity)', it has, therefore, no square root". *Bhaskara*, another Indian mathematician, also writes in his work *Bijaganita*, written in 1150. "There is no square root of a negative quantity, for it is not a square." *Cardan* (1545) considered the problem of solving

$$\infty + \text{y} = 10,\\ \infty \text{y} = 40.$$

He obtained *x* = 5 + −15 and *y = 5 –* −15 as the solution of it, which was discarded by him by saying that these numbers are 'useless'. *Albert Girard* (about 1625) accepted square root of negative numbers and said that this will enable us to get as many roots as the degree of the polynomial equation. *Euler* was the first to introduce the symbol *i* for −1 and *W.R. Hamilton* (about 1830) regarded the complex number *a* + *ib* as an ordered pair of real numbers (*a*, *b*) thus giving it a purely mathematical definition and avoiding use of the so called '*imaginary numbers*'.

**—** v **—**